Small update to xidp

Protocol/SAMLProtocol.fst
@@ -15,9 +15,10 @@ type Assertion =
 
 type SamlMessage =
   | Login: uri -> SamlMessage
+  | LoginResponse: string -> SamlMessage
   | AuthnRequest: issuer:prin ->  destination:endpoint -> message:string -> dsig -> SamlMessage
   | AuthResponseMessage: issuer:prin -> destination:endpoint -> Assertion -> SamlMessage
-  | LoginResponse: string -> SamlMessage
+  | UserCredRequest: challenge:nonce -> SamlMessage
   | Failed: int -> SamlMessage
 
 type SamlStatus =
@@ -27,7 +28,7 @@ type SamlStatus =
 
 
 val SendSaml: prin -> SamlMessage -> unit
-val RecieveSaml: prin -> SamlMessage 
+val ReceiveSaml: prin -> SamlMessage 
 
 val IssuerAssertion: issuer:prin -> subject:prin -> audience:prin -> inresto:id -> assertiontoken
 val AddSignatureToAssertion: assertiontoken -> dsig -> signedtoken
