Protocol/xserver.fst
@@ -8,7 +8,7 @@ open Crypto
 val serviceprovider:  me:prin -> pubkey me -> privkey me ->
                       client:prin -> idp:prin -> pubkey idp -> unit 
 let serviceprovider me pubk privk client idp pubkidp = 
- let req = RecieveSaml client in
+ let req = ReceiveSaml client in
  match req with
   | Login (url) -> (*Create AuthnRequest and send back*)
     let authnReq = CreateAuthnRequestMessage me idp in
@@ -30,36 +30,3 @@ let serviceprovider me pubk privk client idp pubkidp =
       serviceprovider me pubk privk client idp pubkidp (*Start over*)
   | _ -> SendSaml client (Failed 400);(*8.1*)
         serviceprovider me pubk privk client idp pubkidp (*Start over*)
-
-
-
-
-
-(*  let req = Recieve client in (*1*) (*7*)
-  match req with
-  | Get (uri,params,cookies) -> 
-
-    (*Check for valid session*)
-    if hasValidSession cookies then
-      let resp = Response (getContent uri) [] in
-      Send resp (*8*)
-    else (*Create AuthnRequest and send (via client) to idp*)
-      (let authnReq = CreateAuthnRequest me idp in 
-      assume(Log me authnReq) (*Protocol event*);
-      let sigSP = Sign me privk authnReq in
-      let resp = CreateRedirectResponse idp authnReq sigSP in 
-      Send resp (*2*))
-
-  | Post (uri, qparams, fparams, cookies) -> 
-      let msg = getStrInTupleList fparams "SamlMessage" in
-      let sigIDP = getStrInTupleList fparams "Signature" in
-      if VerifySignature idp pubkidp msg sigIDP
-      then
-        (assert(Log idp msg);
-          let ak =  GenerateNonce me in
-          let resp = Response (getContent "Logged-in") [("AuthenticationKey", ak)] in
-          Send resp) (*8*)
-      else Send (ErrorResponse 403 (getErrorPage 403) [])(*8.1*)
-  
-  | _ -> Send (ErrorResponse 400 (getErrorPage 400) [])
-*)
